rename

PsCore.v
@@ -18,35 +18,38 @@ Definition stack : Set := list term.
 
 Definition environment : Set := (stack * stack)%type.
 
-Inductive reduction : relation environment :=
-  | reduction_pop  :
+Inductive eval : relation environment :=
+  | evalpop  :
       forall (t : term) (vs ps : stack),
-      reduction (t :: vs, term_pop :: ps) (vs, ps)
-  | reduction_dup  :
+      eval (t :: vs, term_pop :: ps) (vs, ps)
+  | evaldup  :
       forall (t : term) (vs ps : stack),
-      reduction (t :: vs, term_dup :: ps) (t :: t :: vs, ps)
-  | reduction_swap :
+      eval (t :: vs, term_dup :: ps) (t :: t :: vs, ps)
+  | evalswap :
       forall (t1 t2 : term) (vs ps : stack),
-      reduction (t1 :: t2 :: vs, term_swap :: ps) (t2 :: t1 :: vs, ps)
-  | reduction_cons :
+      eval (t1 :: t2 :: vs, term_swap :: ps) (t2 :: t1 :: vs, ps)
+  | evalcons :
       forall (t1 t2 : term) (vs ps : stack),
-      reduction (t1 :: t2 :: vs, term_cons :: ps) (term_seq t2 t1 :: vs, ps)
-  | reduction_push :
+      eval (t1 :: t2 :: vs, term_cons :: ps) (term_seq t2 t1 :: vs, ps)
+  | evalpush :
       forall (t : term) (vs ps : stack),
-      reduction (vs, term_push :: t :: ps) (t :: vs, ps)
-  | reduction_exec :
+      eval (vs, term_push :: t :: ps) (t :: vs, ps)
+  | evalexec :
       forall (t : term) (vs ps : stack),
-      reduction (t :: vs, term_exec :: ps) (vs, t :: ps)
-  | reduction_seq  :
+      eval (t :: vs, term_exec :: ps) (vs, t :: ps)
+  | evalseq  :
       forall (t1 t2 : term) (vs ps : stack),
-      reduction (vs, term_seq t1 t2 :: ps) (vs, t1 :: t2 :: ps).
+      eval (vs, term_seq t1 t2 :: ps) (vs, t1 :: t2 :: ps).
 
-Definition redstar : relation environment := clos_refl_trans _ reduction.
+Definition evalrts : relation environment := clos_refl_trans _ eval.
+Definition evalrts' : relation environment := clos_refl_trans_1n _ eval.
 
-Definition redstar' : relation environment := clos_refl_trans_1n _ reduction.
+Infix "|=>" := eval (at level 80, no associativity).
+Infix "|=>*" := evalrts (at level 80, no associativity).
+Infix "|=>*'" := evalrts' (at level 80, no associativity).
 
-Lemma decide_reduction : forall (e1 : environment),
-  decidable (exists e2 : environment, reduction e1 e2).
+Lemma decide_eval : forall (e1 : environment),
+  decidable (exists e2 : environment, e1 |=> e2).
   intros.
   destruct e1.
   destruct s0.
@@ -56,31 +59,30 @@ Lemma decide_reduction : forall (e1 : environment),
   destruct t.
   destruct s.
   right ; intro ; destruct H ; inversion H.
-  left ; eexists ; apply reduction_pop.
+  left ; eexists ; apply evalpop.
   destruct s.
   right ; intro ; destruct H ; inversion H.
-  left ; eexists ; apply reduction_dup.
-  destruct s.
-  right ; intro ; destruct H ; inversion H.
-  destruct s.
-  right ; intro ; destruct H ; inversion H.
-  left ; eexists ; apply reduction_swap.
+  left ; eexists ; apply evaldup.
   destruct s.
   right ; intro ; destruct H ; inversion H.
   destruct s.
   right ; intro ; destruct H ; inversion H.
-  left ; eexists ; apply reduction_cons.
+  left ; eexists ; apply evalswap.
+  destruct s.
+  right ; intro ; destruct H ; inversion H.
+  destruct s.
+  right ; intro ; destruct H ; inversion H.
+  left ; eexists ; apply evalcons.
   destruct s0.
   right ; intro ; destruct H ; inversion H.
-  left ; eexists ; apply reduction_push.
+  left ; eexists ; apply evalpush.
   destruct s.
   right ; intro ; destruct H ; inversion H.
-  left ; eexists ; apply reduction_exec.
-  left ; eexists ; apply reduction_seq.
+  left ; eexists ; apply evalexec.
+  left ; eexists ; apply evalseq.
 Defined.
 
-Lemma reduction_unique : forall (a b c : environment),
-  reduction a b -> reduction a c -> b = c.
+Lemma eval_unique : forall (a b c : environment), a |=> b -> a |=> c -> b = c.
   intros.
   destruct a, b, c.
   destruct s0.
@@ -96,26 +98,26 @@ Lemma reduction_unique : forall (a b c : environment),
   inversion H ; inversion H0 ; congruence.
 Qed.
 
-Lemma redstar_confluence : forall (a b c : environment),
-  redstar a b -> redstar a c -> redstar b c \/ redstar c b.
-  unfold redstar.
+Lemma evalrts_confluence :
+  forall (a b c : environment), a |=>* b -> a |=>* c -> b |=>* c \/ c |=>* b.
+  unfold evalrts.
   intros.
-  assert (redstar' a b).
+  assert (a |=>*' b).
     apply clos_rt_rt1n ; auto.
-  assert (redstar' a c).
+  assert (a |=>*' c).
     apply clos_rt_rt1n ; auto.
   induction H1 ; auto.
   inversion H2.
   rewrite <- H4 ; auto.
   apply IHclos_refl_trans_1n.
   apply clos_rt1n_rt ; auto.
-  apply clos_rt1n_rt ; rewrite (reduction_unique _ _ _ H1 H4) ; auto.
-  rewrite (reduction_unique _ _ _ H1 H4) ; auto.
+  apply clos_rt1n_rt ; rewrite (eval_unique _ _ _ H1 H4) ; auto.
+  rewrite (eval_unique _ _ _ H1 H4) ; auto.
 Qed.
 
 Ltac evalstep' e1 e2 :=
   try apply rt_refl ;
-  match eval hnf in (decide_reduction e1) with
+  match eval hnf in (decide_eval e1) with
     | or_introl _ (ex_intro _ ?e3 ?p) =>
       apply (rt_trans _ _ _ _ _ (rt_step _ _ _ _ p))
     | or_intror _ _ => idtac
@@ -124,18 +126,18 @@ Ltac evalstep' e1 e2 :=
 
 Ltac evalstep :=
   match goal with
-    | |- redstar ?e1 ?e2 => evalstep' e1 e2
-    | |- clos_refl_trans _ reduction ?e1 ?e2 => evalstep' e1 e2
+    | |- ?e1 |=>* ?e2 => evalstep' e1 e2
+    | |- clos_refl_trans _ eval ?e1 ?e2 => evalstep' e1 e2
     | _ => fail 2 "The goal is invalid."
   end.
 
 Ltac evalauto := repeat evalstep.
 
-Ltac redpartial t := eapply rt_trans ; [ apply t ; fail | ].
+Ltac evalpartial t := eapply rt_trans ; [ apply t ; fail | ].
 
-Ltac redpartial' t := eapply rt_trans ; [ eapply t | ].
+Ltac evalpartial' t := eapply rt_trans ; [ eapply t | ].
 
-Ltac rtequal :=
+Ltac rtcequal :=
   hnf ;
   match goal with
     | |- clos_refl_trans _ _ ?e1 ?e2 =>
@@ -145,25 +147,25 @@ Ltac rtequal :=
 
 Definition termnop : term := term_seq (term_seq term_push term_pop) term_pop.
 
-Lemma rednop : forall (vs ps : stack), redstar (vs, termnop :: ps) (vs, ps).
+Lemma evalnop : forall (vs ps : stack), (vs, termnop :: ps) |=>* (vs, ps).
   intros ; evalauto.
 Qed.
 
 Definition term_list' : list term -> term -> term := fold_left term_seq.
 
-Lemma red_term_list' : forall (ts : list term) (t : term) (vs ps : stack),
-  redstar (vs, term_list' ts t :: ps) (vs, t :: ts ++ ps).
+Lemma eval_term_list' : forall (ts : list term) (t : term) (vs ps : stack),
+  (vs, term_list' ts t :: ps) |=>* (vs, t :: ts ++ ps).
   induction ts ; intros.
   evalauto.
-  redpartial IHts ; evalauto.
+  evalpartial IHts ; evalauto.
 Qed.
 
 Definition term_list (ts : list term) : term := term_list' ts termnop.
 
-Lemma red_term_list : forall (ts : list term) (vs ps : stack),
-  redstar (vs, term_list ts :: ps) (vs, ts ++ ps).
+Lemma eval_term_list : forall (ts : list term) (vs ps : stack),
+  (vs, term_list ts :: ps) |=>* (vs, ts ++ ps).
   intros.
-  redpartial red_term_list'.
+  evalpartial eval_term_list'.
   evalauto.
 Qed.
 
@@ -188,14 +190,14 @@ Qed.
 
 Definition term_snoc : term := term_list [ term_swap ; term_cons ].
 
-Lemma red_snoc : forall (t1 t2 : term) (vs ps : stack),
-  redstar (t1 :: t2 :: vs, term_snoc :: ps) (term_seq t1 t2 :: vs, ps).
+Lemma evalsnoc : forall (t1 t2 : term) (vs ps : stack),
+  (t1 :: t2 :: vs, term_snoc :: ps) |=>* (term_seq t1 t2 :: vs, ps).
   intros ; evalauto.
 Qed.
 
 Definition term_quote : term := term_list [term_push ; term_push ; term_snoc ].
 
 Lemma red_term_quote : forall (t : term) (vs ps : stack),
-  redstar (t :: vs, term_quote :: ps) (term_seq term_push t :: vs, ps).
+  (t :: vs, term_quote :: ps) |=>* (term_seq term_push t :: vs, ps).
   intros ; evalauto.
 Qed.
